theories/persistently.v
@@ -427,7 +427,8 @@ Proof.
   *)
   1, 2: wp_load; by iFrame.
   (** The threads return their fractions. *)
-  iIntros (v1 v2) "[[-> Hl1] [-> Hl2]] !>".
+  iIntros (v1 v2) "[[-> Hl1] [-> Hl2]]".
+  iNext.
   wp_let.
   (** We combine them, allowing us to perform the store. *)
   iCombine "Hl1 Hl2" as "Hl".
@@ -494,7 +495,8 @@ Proof.
   wp_pures.
   wp_apply (wp_par t_post t_post).
   1, 2: wp_load; wp_pures; done.
-  iIntros (v1 v2) "[-> ->] !>".
+  iIntros (v1 v2) "[-> ->]".
+  iNext.
   wp_pures.
   by iApply "HΦ".
 Qed.
